Games/gameLib/Basic.lean
@@ -954,7 +954,7 @@ played is won by the first player.
 def Game_World.is_fst_win  {α β : Type u} (g : Game_World α β) : Prop :=
   ∃ ws : Strategy α β,
   ∀ snd_s : Strategy α β,
-  ∃ ws_leg : Strategy_legal_fst g.init_game_state (fun _ => g.fst_legal) ws snd_s,
+   (ws_leg : Strategy_legal_fst g.init_game_state (fun _ => g.fst_legal) ws snd_s) →
    (snd_leg : Strategy_legal_snd g.init_game_state (fun _ => g.snd_legal) ws snd_s) →
   ({g with fst_strat := ws, fst_lawful := ws_leg, snd_strat := snd_s, snd_lawful := snd_leg} : Game α β).fst_win
 
@@ -967,7 +967,7 @@ played is won by the second player.
 def Game_World.is_snd_win  {α β : Type u} (g : Game_World α β) : Prop :=
   ∃ ws : Strategy α β,
   ∀ fst_s : Strategy α β,
-  ∃ ws_leg : Strategy_legal_snd g.init_game_state (fun _ => g.snd_legal) fst_s ws,
+   (ws_leg : Strategy_legal_snd g.init_game_state (fun _ => g.snd_legal) fst_s ws) →
    (fst_leg : Strategy_legal_fst g.init_game_state (fun _ => g.fst_legal) fst_s ws) →
   ({g with fst_strat := fst_s, fst_lawful := fst_leg, snd_strat := ws, snd_lawful := ws_leg} : Game α β).snd_win
 
@@ -984,7 +984,7 @@ def Symm_Game.snd_win  {α β : Type u} (g : Symm_Game α β) : Prop :=
 def Symm_Game_World.is_fst_win  {α β : Type u} (g : Symm_Game_World α β) : Prop :=
   ∃ ws : Strategy α β,
   ∀ snd_s : Strategy α β,
-  ∃ ws_leg : Strategy_legal_fst g.init_game_state (fun _ => g.law) ws snd_s,
+   (ws_leg : Strategy_legal_fst g.init_game_state (fun _ => g.law) ws snd_s) →
    (snd_leg : Strategy_legal_snd g.init_game_state (fun _ => g.law) ws snd_s) →
   ({g with fst_strat := ws, fst_lawful := ws_leg, snd_strat := snd_s, snd_lawful := snd_leg} : Symm_Game α β).fst_win
 
@@ -992,7 +992,7 @@ def Symm_Game_World.is_fst_win  {α β : Type u} (g : Symm_Game_World α β) : P
 def Symm_Game_World.is_snd_win  {α β : Type u} (g : Symm_Game_World α β) : Prop :=
   ∃ ws : Strategy α β,
   ∀ fst_s : Strategy α β,
-  ∃ ws_leg : Strategy_legal_snd g.init_game_state (fun _ => g.law) fst_s ws,
+   (ws_leg : Strategy_legal_snd g.init_game_state (fun _ => g.law) fst_s ws) →
    (fst_leg : Strategy_legal_fst g.init_game_state (fun _ => g.law) fst_s ws ) →
   ({g with fst_strat := fst_s, fst_lawful := fst_leg, snd_strat := ws, snd_lawful := ws_leg} : Symm_Game α β).snd_win
 
@@ -1022,7 +1022,7 @@ played is won by the first player.
 def Game_World_wDraw.is_fst_win  {α β : Type u} (g : Game_World_wDraw α β) : Prop :=
   ∃ ws : Strategy α β,
   ∀ snd_s : Strategy α β,
-  ∃ ws_leg : Strategy_legal_fst g.init_game_state (fun _ => g.fst_legal) ws snd_s,
+   (ws_leg : Strategy_legal_fst g.init_game_state (fun _ => g.fst_legal) ws snd_s) →
    (snd_leg : Strategy_legal_snd g.init_game_state (fun _ => g.snd_legal) ws snd_s) →
   ({g with fst_strat := ws, fst_lawful := ws_leg, snd_strat := snd_s, snd_lawful := snd_leg} : Game α β).fst_win
 
@@ -1035,7 +1035,7 @@ played is won by the second player.
 def Game_World_wDraw.is_snd_win  {α β : Type u} (g : Game_World_wDraw α β) : Prop :=
   ∃ ws : Strategy α β,
   ∀ fst_s : Strategy α β,
-  ∃ ws_leg : Strategy_legal_snd g.init_game_state (fun _ => g.snd_legal) fst_s ws,
+   (ws_leg : Strategy_legal_snd g.init_game_state (fun _ => g.snd_legal) fst_s ws) →
    (fst_leg : Strategy_legal_fst g.init_game_state (fun _ => g.fst_legal) fst_s ws) →
   ({g with fst_strat := fst_s, fst_lawful := fst_leg, snd_strat := ws, snd_lawful := ws_leg} : Game α β).snd_win
 
@@ -1043,7 +1043,7 @@ def Game_World_wDraw.is_snd_win  {α β : Type u} (g : Game_World_wDraw α β) :
 def Game_World_wDraw.is_fst_draw  {α β : Type u} (g : Game_World_wDraw α β) : Prop :=
   ∃ ws : Strategy α β,
   ∀ snd_s : Strategy α β,
-  ∃ ws_leg : Strategy_legal_fst g.init_game_state (fun _ => g.fst_legal) ws snd_s,
+   (ws_leg : Strategy_legal_fst g.init_game_state (fun _ => g.fst_legal) ws snd_s) →
    (snd_leg : Strategy_legal_snd g.init_game_state (fun _ => g.snd_legal) ws snd_s) →
   ({g with fst_strat := ws, fst_lawful := ws_leg, snd_strat := snd_s, snd_lawful := snd_leg} : Game_wDraw α β).fst_draw
 
@@ -1051,7 +1051,7 @@ def Game_World_wDraw.is_fst_draw  {α β : Type u} (g : Game_World_wDraw α β) 
 def Game_World_wDraw.is_snd_draw  {α β : Type u} (g : Game_World_wDraw α β) : Prop :=
   ∃ ws : Strategy α β,
   ∀ fst_s : Strategy α β,
-  ∃ ws_leg : Strategy_legal_snd g.init_game_state (fun _ => g.snd_legal) fst_s ws,
+   (ws_leg : Strategy_legal_snd g.init_game_state (fun _ => g.snd_legal) fst_s ws) →
    (fst_leg : Strategy_legal_fst g.init_game_state (fun _ => g.fst_legal) fst_s ws) →
   ({g with fst_strat := fst_s, fst_lawful := fst_leg, snd_strat := ws, snd_lawful := ws_leg} : Game_wDraw α β).snd_draw
 
